clean up

negations/nsubtyping.v
@@ -1,4 +1,4 @@
-Require Import ST.src.stream ST.processes.process ST.src.st ST.src.so ST.src.si ST.src.reordering 
+Require Import ST.src.stream ST.src.st ST.src.so ST.src.si ST.src.reordering 
                ST.src.siso ST.types.local ST.subtyping.refinement ST.src.reorderingfacts 
                ST.subtyping.subtyping ST.negations.nrefinement.
 From mathcomp Require Import all_ssreflect seq ssrnat.
@@ -9,80 +9,15 @@ Require Import Setoid.
 Require Import Morphisms.
 Require Import Coq.Logic.Classical_Pred_Type  Coq.Logic.ClassicalFacts Coq.Logic.Classical_Prop.
 
-Locate extdpn.
-
-Fixpoint listSisoNRef (l: list (siso*siso)): Prop :=
-  match l with
-    | nil            => False
-    | cons (W,W') xs => (forall d1, forall d2, (exists n, (nRefinement (mk_siso (merge_dpf_contn d1 (@und W) n) (extdpfn (@und W) (@sprop W)))
-                                                                       (mk_siso (merge_dpf_contn d2 (@und W') n) (extdpfn (@und W') (@sprop W'))))))
-                        \/ listSisoNRef xs
-  end.
-
-Definition nsubtype (T T': st): Prop := forall (l: list (siso*siso)), decomposeL l T T' -> listSisoNRef l.
-
-(* Definition nsubltype (T T': local) (T1 T2: st) (P: lt2stC T T1) (Q: lt2stC T' T2 ) := nsubtype T1 T2. *)
-
-Lemma trivL2:  forall l, (listSisoPRef2 l -> False) -> listSisoNRef l.
-Proof. intro l.
-       induction l; intros.
-       - simpl in *. easy.
-       - simpl in *. destruct a as (W, W').
-         destruct W as (w, Hw).
-         destruct W' as (w', Hw').
-         apply not_and_or in H.
-         destruct H as [H| H].
-         left.
-         intros d1 d2.
-         apply not_ex_all_not with (n := d1) in H.
-         apply not_ex_all_not with (n := d2) in H.
-         apply not_all_ex_not in H.
-         destruct H as (n, H).
-         exists n.
-         apply nRefL.
-         intros.
-         apply H.
-         simpl in *.
-         rewrite <- !meqDpf in H, H0. easy.
-         right.
-         apply IHl. easy.
-Qed.
-
-Lemma trivL1: forall l, listSisoPRef2 l -> listSisoNRef l -> False.
-Proof. intro l.
-       induction l; intros.
-       - simpl in *. easy.
-       - simpl in *. destruct a as (W, W').
-         destruct W as (w, Hw).
-         destruct W' as (w', Hw').
-         destruct H as ((d1,(d2,Ha)), Hb).
-         destruct H0 as [H0 | H0].
-         specialize(H0 d1 d2).
-         destruct H0 as (n, H0).
-         specialize(Ha n).
-         simpl in H0.
-         specialize (nRefR ({| und := merge_dpf_contn d1 w n; sprop := extdpfn w Hw |}) ( {| und := merge_dpf_contn d2 w' n; sprop := extdpfn w' Hw' |})); intros.
-         apply H. easy.
-         easy.
-         apply IHl. easy. easy.
-Qed.
-
-(*talk*)
-Definition subtype3 (T T': st): Prop :=
-  forall U, st2soC T U /\ 
-  forall V', st2siC T' V' /\
-  exists (W: siso), st2sisoC U  (@und W) /\
-  exists (W':siso), st2sisoC V' (@und W') /\ (@und W) ~< (@und W').
-
-Definition nsubtype3 (T T': st): Prop :=
+Definition nsubtype (T T': st): Prop :=
   exists U,  (st2soC T U) ->
   exists V', (st2siC T' V') ->
   forall W,  (st2sisoC U (@und W)) ->
   forall W', (st2sisoC V' (@und W')) -> nRefinement W W'.
 
-Lemma subNeq3L: forall T T', (subtype3 T T' -> False) -> nsubtype3 T T'.
+Lemma subNeqL: forall T T', (subtype T T' -> False) -> nsubtype T T'.
 Proof. intros.
-       unfold subtype3, nsubtype3 in *.
+       unfold subtype, nsubtype in *.
        apply not_all_ex_not in H.
        destruct H as (U, H).
        exists U.
@@ -112,9 +47,9 @@ Proof. intros.
        apply nRefL. easy.
 Qed.
 
-Lemma subNeq3R: forall T T', nsubtype3 T T' -> (subtype3 T T' -> False).
+Lemma subNeqR: forall T T', nsubtype T T' -> (subtype T T' -> False).
 Proof. intros.
-       unfold subtype3, nsubtype3 in *.
+       unfold subtype, nsubtype in *.
        rename H into Ha.
        rename H0 into H.
        rename Ha into H0.
