subtyping/refinement.v
@@ -9,27 +9,17 @@ Require Import Morphisms.
 Inductive refinementR (seq: st -> st -> Prop): st -> st -> Prop :=
   | ref_a  : forall w w' p l s s' a n, subsort s' s ->
                                        seq w (merge_ap_contn p a w' n)  ->
-                                       ( exists L1, exists L2,
-                                         coseqInLC (act w) L1 /\
-                                         coseqInLC (act (merge_ap_contn p a w' n)) L2 /\
-                                         coseqInR L1 (act w) /\
-                                         coseqInR L2 (act (merge_ap_contn p a w' n)) /\
-                                         (forall x, List.In x L1 <-> List.In x L2)
-                                        ) ->
+                                       act_eq w (merge_ap_contn p a w' n) ->
                                        refinementR seq (st_receive p (cocons (l,s,w) conil)) (merge_ap_contn p a (st_receive p (cocons (l,s',w') conil)) n)
   | ref_b  : forall w w' p l s s' b n, subsort s s' ->
                                        seq w (merge_bp_contn p b w' n) ->
-                                       ( exists L1, exists L2,
-                                         coseqInLC (act w) L1 /\
-                                         coseqInLC (act (merge_bp_contn p b w' n)) L2 /\
-                                         coseqInR L1 (act w) /\
-                                         coseqInR L2 (act (merge_bp_contn p b w' n)) /\
-                                         (forall x, List.In x L1 <-> List.In x L2)
-                                       ) ->
+                                       act_eq w (merge_bp_contn p b w' n) ->
                                        refinementR seq (st_send p (cocons (l,s,w) conil)) (merge_bp_contn p b (st_send p (cocons (l,s',w') conil)) n)
   | ref_end: refinementR seq st_end st_end.
 
 Definition refinement: st -> st -> Prop := fun s1 s2 => paco2 refinementR bot2 s1 s2.
+
+Notation "x '~<' y" := (refinement x y) (at level 50, left associativity).
 
 Lemma refinementR_mon: monotone2 refinementR.
 Proof. unfold monotone2.
@@ -42,73 +32,3 @@ Proof. unfold monotone2.
        - constructor.
 Qed.
 
-(* the second refinement *)
-
-Inductive refinementR2 (seq: st -> st -> Prop): st -> st -> Prop :=
-  | ref2_a  : forall w w' p l s s' a n, subsort s' s ->
-                                        seq w (merge_ap_contn p a w' n)  ->
-                                        act_eq w (merge_ap_contn p a w' n) ->
-                                        refinementR2 seq (st_receive p (cocons (l,s,w) conil)) (merge_ap_contn p a (st_receive p (cocons (l,s',w') conil)) n)
-  | ref2_b  : forall w w' p l s s' b n, subsort s s' ->
-                                        seq w (merge_bp_contn p b w' n) ->
-                                        act_eq w (merge_bp_contn p b w' n) ->
-                                        refinementR2 seq (st_send p (cocons (l,s,w) conil)) (merge_bp_contn p b (st_send p (cocons (l,s',w') conil)) n)
-  | ref2_end: refinementR2 seq st_end st_end.
-
-Definition refinement2: st -> st -> Prop := fun s1 s2 => paco2 refinementR2 bot2 s1 s2.
-
-Notation "x '~<' y" := (refinement2 x y) (at level 50, left associativity).
-
-Lemma refinementR2_mon: monotone2 refinementR2.
-Proof. unfold monotone2.
-       intros.
-       induction IN; intros.
-       - specialize(ref2_a r'); intro Ha. apply Ha; try easy.
-         apply LE. exact H0.
-       - specialize(ref2_b r'); intro Ha. apply Ha; try easy.
-         apply LE. exact H0.
-       - constructor.
-Qed.
-
-(* #[export]
-Declare Instance Ref_Trans: Transitive (refinement). *)
-
-Inductive refinementR3 (seq: st -> st -> Prop): st -> st -> Prop :=
-  | ref3_a  : forall w w' p l s s' a n, subsort s' s ->
-                                        isInA a p = false ->
-                                        seq w (merge_apf_contn a w' n)  -> 
-                                        ( exists L1, exists L2,
-                                          coseqInLC (act w) L1 /\
-                                          coseqInLC (act (merge_apf_contn a w' n)) L2 /\
-                                          coseqInR L1 (act w) /\
-                                          coseqInR L2 (act (merge_apf_contn a w' n)) /\
-                                          (forall x, List.In x L1 <-> List.In x L2)
-                                         ) ->
-(*                                         act_eq w (merge_apf_contn a w' n) -> *)
-                                        refinementR3 seq (st_receive p (cocons (l,s,w) conil)) (merge_apf_contn a (st_receive p (cocons (l,s',w') conil)) n)
-  | ref3_b  : forall w w' p l s s' b n, subsort s s' ->
-                                        isInB b p = false ->
-                                        seq w (merge_bpf_contn b w' n) -> 
-                                        ( exists L1, exists L2,
-                                          coseqInLC (act w) L1 /\
-                                          coseqInLC (act (merge_bpf_contn b w' n)) L2 /\
-                                          coseqInR L1 (act w) /\
-                                          coseqInR L2 (act (merge_bpf_contn b w' n)) /\
-                                          (forall x, List.In x L1 <-> List.In x L2)
-                                        ) ->
-(*                                         act_eq w (merge_bpf_contn b w' n) -> *)
-                                        refinementR3 seq (st_send p (cocons (l,s,w) conil)) (merge_bpf_contn b (st_send p (cocons (l,s',w') conil)) n)
-  | ref3_end: refinementR3 seq st_end st_end.
-
-Definition refinement3: st -> st -> Prop := fun s1 s2 => paco2 refinementR3 bot2 s1 s2.
-
-Lemma refinementR3_mon: monotone2 refinementR3.
-Proof. unfold monotone2.
-       intros.
-       induction IN; intros.
-       - specialize(ref3_a r'); intro Ha. apply Ha; try easy.
-         apply LE. exact H1. 
-       - specialize(ref3_b r'); intro Ha. apply Ha; try easy.
-         apply LE. exact H1.
-       - constructor.
-Qed.
