subtyping/subtyping.v
@@ -9,38 +9,12 @@ Require Import Morphisms.
 Require Import Coq.Logic.Classical_Pred_Type Coq.Logic.ClassicalFacts Coq.Logic.Classical_Prop.
 Require Import ProofIrrelevance.
 
-Fixpoint listSisoPRef (l: list (siso*siso)): Prop :=
-  match l with
-    | nil            => True
-    | cons (W,W') xs => (exists d1, exists d2, (forall n, refinement (merge_dpf_contn d1 (@und W) n) (merge_dpf_contn d2 (@und W') n))) /\ listSisoPRef xs
-  end.
-
-Fixpoint decomposeL (l: list (siso*siso)) (s: st) (s': st): Prop :=
-  match l with
-    | nil            => True
-    | cons (W,W') xs => st2sisoC (@und W) s /\ st2sisoC (@und W') s' /\ decomposeL xs s s'
-  end.
-
-Definition subtype (T T': st): Prop := exists (l: list (siso*siso)), decomposeL l T T' /\ listSisoPRef l.
-
-Fixpoint listSisoPRef2 (l: list (siso*siso)): Prop :=
-  match l with
-    | nil            => True
-    | cons (W,W') xs => (exists d1, exists d2, (forall n, (merge_dpf_contn d1 (@und W) n) ~<  (merge_dpf_contn d2 (@und W') n))) /\ listSisoPRef2 xs
-  end.
-
-Definition subtype2 (T T': st): Prop := exists (l: list (siso*siso)), decomposeL l T T' /\ listSisoPRef2 l.
-
-(* Fixpoint listSisoPRef3A (l: list (siso*siso)): Prop :=
-  match l with
-    | nil            => True
-    | cons (W,W') xs => (exists b1, exists b2, (forall n, refinement3 (merge_bpf_contn b1 (@und W) n)  (merge_bpf_contn b2 (@und W') n))) /\ listSisoPRef3A xs
-  end.
-
-Definition subtype3A (T T': st): Prop := exists (l: list (siso*siso)), decomposeL l T T' /\ listSisoPRef3A l. *)
+Definition subtype (T T': st): Prop :=
+  forall U, st2soC T U /\ 
+  forall V', st2siC T' V' /\
+  exists (W: siso), st2sisoC U  (@und W) /\
+  exists (W':siso), st2sisoC V' (@und W') /\ (@und W) ~< (@und W').
 
 Definition subltype (T T': local) := subtype (lt2st T) (lt2st T').
-
-(* Definition subltype2 (T T': local) (T1 T2: st) (P: lt2stC T T1) (Q: lt2stC T' T2) := subtype2 T1 T2. *)
 
 
